theories/VLSM/Core/Validator.v
@@ -94,7 +94,7 @@ Context
   (Htransition_None : weak_projection_transition_consistency_None _ _ label_project state_project)
   (label_lift : vlabel Y -> vlabel X)
   (state_lift : vstate Y -> vstate X)
-  (Xi := projection_induced_vlsm X (type Y) label_project state_project label_lift state_lift)
+  (Xi := pre_projection_induced_vlsm X (type Y) label_project state_project label_lift state_lift)
   (Hlabel_lift : induced_projection_label_lift_prop _ _ label_project label_lift)
   (Hstate_lift : induced_projection_state_lift_prop _ _ state_project state_lift)
   (Hinitial_lift : strong_full_projection_initial_state_preservation Y X state_lift)
@@ -126,16 +126,12 @@ Lemma induced_projection_incl_preloaded_with_all_messages
   : VLSM_incl Xi PreY.
 Proof.
   apply basic_VLSM_incl.
-  - intros is (s & <- & Hs).
-    by apply (VLSM_projection_initial_state Hproj).
-  - intros l s m Hv HsY HmX. apply any_message_is_valid_in_preloaded.
-  - intros l s om (_ & _ & lX & sX & Hlx & <- & Hv) _ _.
-    simpl.
-    by eapply (VLSM_projection_input_valid Hproj).
-  - intros l s im s' om [[_ [_ HvXi]] HtXi].
-    setoid_rewrite <- HtXi.
-    symmetry.
-    by apply projection_induced_valid_transition_eq.
+  - by intros is (s & <- & Hs); apply (VLSM_projection_initial_state Hproj).
+  - by intros l s m Hv HsY HmX; apply initial_message_is_valid.
+  - by intros l s om (_ & _ & lX & sX & Hlx & <- & Hv) _ _
+    ; simpl; eapply VLSM_projection_input_valid.
+  - intros l s im s' om [[_ [_ HvXi]] HtXi]; cbn.
+    by setoid_rewrite <- HtXi; rewrite <- projection_induced_valid_transition_eq.
 Qed.
 
 (** An alternative formulation of the [projection_validator_prop]erty with a
@@ -328,17 +324,14 @@ Lemma pre_loaded_with_all_messages_validator_component_proj_eq
   (Hvalidator : component_projection_validator_prop)
   : VLSM_eq PreXi Xi.
 Proof.
-  apply VLSM_eq_trans with
-    (machine (projection_induced_vlsm X (type (IM i))
-      (composite_project_label IM i) (fun s => s i)
-      (lift_to_composite_label IM i) (lift_to_composite_state' IM i)))
-  ; simpl; [|apply VLSM_eq_sym, composite_vlsm_constrained_projection_is_induced].
+  eapply VLSM_eq_trans;
+    [| apply VLSM_eq_sym, composite_vlsm_constrained_projection_is_induced].
   apply pre_loaded_with_all_messages_validator_proj_eq.
   - apply component_projection_to_preloaded.
   - apply component_transition_projection_None.
   - apply component_label_projection_lift.
   - apply component_state_projection_lift.
-  - intro s. apply (composite_initial_state_prop_lift IM).
+  - intro s; apply (composite_initial_state_prop_lift IM).
   - apply component_transition_projection_Some.
   - intros li si omi Hiv.
     apply Hvalidator in Hiv as (sX & <- & HivX).
